cleanup and more example

theories/coroutine.v
@@ -10,108 +10,86 @@ Require Import refframe.imp.
 Require Import refframe.asm.
 Require Import refframe.itree.
 Require Import refframe.imp_to_asm.
-Require Import refframe.compiler.compiler.
 
 Local Open Scope Z_scope.
 
-(***
-void gtyield(void)
-{
-	struct gt *old, *new;
-
-	old = &gttbl[gtcur];
-        gtcur = (gtcur+1)%2; // rand()%2;
-	new = &gttbl[gtcur];
-	gtswtch(old, new);
-}
-
-gtswtch.s
-        mov     %rsp, 0x00(%rdi)
-        mov     %r15, 0x08(%rdi)
-        mov     %r14, 0x10(%rdi)
-        mov     %r13, 0x18(%rdi)
-        mov     %r12, 0x20(%rdi)
-        mov     %rbx, 0x28(%rdi)
-        mov     %rbp, 0x30(%rdi)
-
-        mov     0x00(%rsi), %rsp
-        mov     0x08(%rsi), %r15
-        mov     0x10(%rsi), %r14
-        mov     0x18(%rsi), %r13
-        mov     0x20(%rsi), %r12
-        mov     0x28(%rsi), %rbx
-        mov     0x30(%rsi), %rbp
-
-        ret
-***)
-
 Local Coercion ImmediateOp: Z >-> asm_operand.
 Local Coercion RegisterOp: string >-> asm_operand.
-
 
 Definition yield_addr : Z := 2000.
 
 Definition coro_state_addr : Z := 3000.
 
-(*
-Definition yield_asm: gmap Z asm_instr := deep_to_asm_instrs yield_addr
-  [Amov "R9" 0;
-   (** basic setup **)
-   (* R17 := gtcur *)
-   (* Aload "R17" "R9" (gtcur); *)
-   (* R16 := gtnext *)
-   Aslt "R16" "R17" 1;
-
-   (* R15 := gttbl[gtcur] *)
-   Amul "R9" "R17" 13;
-   (* Aadd "R15" "R9" (gttbl); *)
-   (* R14 := gttbl[gtnext] *)
-   Amul "R9" "R16" 13;
-   (* Aadd "R14" "R9" (gttbl); *)
-
-
-   (** store registers to gttbl[gtcur] **)
-   Astore "R19" "R15" 0;
-   Astore "R20" "R15" 1;
-   Astore "R21" "R15" 2;
-   Astore "R22" "R15" 3;
-   Astore "R23" "R15" 4;
-   Astore "R24" "R15" 5;
-   Astore "R25" "R15" 6;
-   Astore "R26" "R15" 7;
-   Astore "R27" "R15" 8;
-   Astore "R28" "R15" 9;
-   Astore "R29" "R15" 10;
-   Astore "R30" "R15" 11;
-   Astore "SP"  "R15" 12;
-
-   (** load gttbl[gtnext] to registers **)
-   Aload "R19" "R14" 0;
-   Aload "R20" "R14" 1;
-   Aload "R21" "R14" 2;
-   Aload "R22" "R14" 3;
-   Aload "R23" "R14" 4;
-   Aload "R24" "R14" 5;
-   Aload "R25" "R14" 6;
-   Aload "R26" "R14" 7;
-   Aload "R27" "R14" 8;
-   Aload "R28" "R14" 9;
-   Aload "R29" "R14" 10;
-   Aload "R30" "R14" 11;
-   Aload "SP"  "R14" 12;
-
-
-   (** argument passing **)
-   (** already handled; argument 0 register == return register == R0 **)
-   (* Amov "R1" "R0"; *)
-   (* Aload "R0" "R9" (yield_val); *)
-   (* Astore "R1" "R9" (yield_val); *)
-
-   Aret]
-.
-*)
-
 Definition coro_saved_regs : list string := "PC"::saved_registers.
+
+Definition coro_get_regs (regs : gmap string Z) : list Z :=
+  ((regs !!!.) <$> coro_saved_regs).
+Arguments coro_get_regs : simpl never.
+
+Definition coro_regs_mem (regs : gmap string Z) : gmap Z (option Z) :=
+  map_seqZ coro_state_addr (Some <$> coro_get_regs regs).
+Arguments coro_regs_mem : simpl never.
+
+Definition coro_regs_regs (regs : gmap string Z) : gmap string Z :=
+  list_to_map ((λ x, (x, regs !!! x)) <$> coro_saved_regs).
+Arguments coro_regs_regs : simpl never.
+
+Lemma coro_regs_regs_args_preserved rs rs':
+ map_preserved args_registers rs (coro_regs_regs rs' ∪ rs).
+Proof.
+  rewrite /coro_regs_regs. cbn.
+  rewrite -!insert_union_l left_id_L.
+  repeat (apply map_preserved_insert_r_not_in; [compute_done|]).
+  done.
+Qed.
+
+Lemma coro_regs_regs_touched_scramble rs rs' rs'':
+  map_scramble touched_registers rs rs' →
+  map_scramble touched_registers rs (coro_regs_regs rs'' ∪ rs').
+Proof.
+  move => ?.
+  rewrite /coro_regs_regs. cbn.
+  rewrite -!insert_union_l left_id_L.
+  repeat (apply map_scramble_insert_r_in; [compute_done|]).
+  done.
+Qed.
+
+Lemma coro_regs_regs_saved_preserved rs rs' rs'':
+  map_preserved saved_registers rs rs'' →
+  map_preserved saved_registers rs (coro_regs_regs rs'' ∪ rs').
+Proof.
+  move => Hp. rewrite /coro_regs_regs. cbn.
+  rewrite -!insert_union_l left_id_L.
+  apply map_preserved_insert_r_not_in; [compute_done|].
+  repeat (apply map_preserved_insert_r_in; [compute_done|]; split; [apply: Hp; compute_done|]).
+  apply map_preserved_nil'. compute_done.
+Qed.
+
+Lemma coro_regs_mem_dom rs rs':
+  dom (gset Z) (coro_regs_mem rs) = dom (gset Z) (coro_regs_mem rs').
+Proof.
+  rewrite /coro_regs_mem/coro_get_regs. cbn. rewrite !dom_insert_L. done.
+Qed.
+
+Lemma coro_regs_regs_lookup_in r rs rs' :
+  r ∈ "PC"::saved_registers →
+  (coro_regs_regs rs ∪ rs') !!! r = rs !!! r.
+Proof.
+  move => ?. set_unfold. rewrite /coro_regs_regs. cbn.
+  rewrite -!insert_union_l left_id_L.
+  destruct_all?; simplify_eq.
+  all: repeat (rewrite lookup_total_insert_ne; [|done]).
+  all: by rewrite lookup_total_insert.
+Qed.
+
+Lemma coro_regs_regs_lookup_not_in r rs rs' :
+  r ∉ "PC"::saved_registers →
+  (coro_regs_regs rs ∪ rs') !!! r = rs' !!! r.
+Proof.
+  move => ?. set_unfold. rewrite /coro_regs_regs. cbn.
+  rewrite -!insert_union_l left_id_L.
+  by repeat (rewrite lookup_total_insert_ne; [|naive_solver]).
+Qed.
 Opaque coro_saved_regs.
 
 Definition yield_swap_reg (r : string) (o : Z) : list deep_asm_instr := [
@@ -128,29 +106,7 @@ Definition yield_asm: gmap Z asm_instr := deep_to_asm_instrs yield_addr (
   Astore "R30" "R17" (Z.of_nat $ length saved_registers);
   Abranch true "R16"]).
 
-Definition coro_get_regs (regs : gmap string Z) : list Z :=
-  ((regs !!!.) <$> coro_saved_regs).
-Arguments coro_get_regs : simpl never.
-
-Definition coro_regs_mem (regs : gmap string Z) : gmap Z (option Z) :=
-  map_seqZ coro_state_addr (Some <$> coro_get_regs regs).
-Arguments coro_regs_mem : simpl never.
-
-Definition coro_regs_regs (regs : gmap string Z) : gmap string Z :=
-  list_to_map ((λ x, (x, regs !!! x)) <$> coro_saved_regs).
-Arguments coro_regs_regs : simpl never.
-
-Lemma coro_regs_regs_lookup_in r rs rs' :
-  r ∈ "PC"::saved_registers →
-  (coro_regs_regs rs ∪ rs') !!! r = rs !!! r.
-Proof.
-Admitted.
-
-Lemma coro_regs_regs_lookup_not_in r rs rs' :
-  r ∉ "PC"::saved_registers →
-  (coro_regs_regs rs ∪ rs') !!! r = rs' !!! r.
-Proof.
-Admitted.
+Definition yield_asm_dom : gset Z := locked (dom _) yield_asm.
 
 Definition yield_itree : itree (moduleE asm_event (gmap string Z)) unit :=
   ITree.forever (
@@ -198,129 +154,12 @@ Proof.
   tstep_i. simplify_map_eq'.
 Admitted.
 
-(***
-int
-gtgo(void *f)
-{
-	struct gt *p;
-
-        p = &gttbl[1];
-
-	/* *&stack[StackSize -  8] = (uint64_t)gtstop; */
-	*&stack[StackSize - 16] = (uint64_t)f;
-	p->rsp = (uint64_t)&stack[StackSize - 16];
-
-	return 0;
-}
-***)
-
-(** simply set p->rsp to be stack, p->pc to be the function **)
-(*
-Definition gtgo_addr: Z := 200.
-
-Definition gtgo_asm: gmap Z asm_instr := deep_to_asm_instrs gtgo_addr
-  [
-    Amov "R9" 0;
-    (*** rsp ***)
-    Amov "R10" (stack + stksize);
-    Astore "R10" "R9" (gttbl + 13 + 12);
-
-    (*** PC ***)
-    Astore "R0" "R9" (gttbl + 13 + 11);
-    Aret
-  ]
-.
-*)
-
-
-(***
-void stream_inner(int n) {
-  gtyield_with_val(n);
-  stream_inner(n+1);
-}
-
-void stream()
-{
-  stream_inner(0);
-}
-
-int main(void)
-{
-  gtgo(stream);
-  for(int i=0; i<5; i++) {
-    int v = gtyield_with_val(-1);
-    printf("v is : %d\n", v);
-  }
-}
-***)
-
-Definition stream_addr: Z := 400.
-Definition main_addr: Z := 500.
-Definition print_addr: Z := 600.
-
-Definition stream_imp: fndef := {|
-  fd_args := [("n")];
-  fd_vars := [];
-  fd_body := LetE "_" (imp.Call "yield" [Var "n"]) $
-             (imp.Call "stream" [(BinOp (Var "n") AddOp (Val $ ValNum 1))]);
-  fd_static := I
-|}.
-
-Definition main_imp: fndef := {|
-  fd_args := [];
-  fd_vars := [("x", -1); ("y", -1)];
-  fd_body := LetE "x" (imp.Call "yield" [Val $ ValNum 0]) $
-             LetE "_" (imp.Call "print" [(Var "x")]) $
-             LetE "y" (imp.Call "yield" [Val $ ValNum 0]) $
-             LetE "_" (imp.Call "print" [(Var "y")]) $
-             (Val $ ValNum (-1));
-  fd_static := I
-|}.
-
-Definition all_f2i : gmap string Z :=
-  <["yield"  := yield_addr]> $
-  <["stream" := stream_addr]> $
-  <["main"   := main_addr]> $
-  <["print"  := print_addr]> $
-  ∅.
-
-Definition stream_asm : gmap Z asm_instr :=
-  deep_to_asm_instrs stream_addr ltac:(i2a_compile all_f2i stream_imp).
-
-Definition main_asm : gmap Z asm_instr :=
-  deep_to_asm_instrs main_addr ltac:(i2a_compile all_f2i main_imp).
-
-Lemma stream_asm_refines_imp :
-  trefines (MS asm_module (initial_asm_state stream_asm))
-           (MS (imp_to_asm (dom _ stream_asm) {["stream"]} all_f2i imp_module)
-               (initial_imp_to_asm_state ∅ imp_module (initial_imp_state (<["stream" := stream_imp]> ∅)))).
-Proof.
-  apply: compile_correct; [|done|..].
-  - by vm_compute.
-  - by vm_compute.
-  - move => ??. rewrite /all_f2i !lookup_insert_Some !lookup_empty.
-    move => ?. destruct_all?; simplify_eq; compute_done.
-Qed.
-
-Lemma main_asm_refines_imp :
-  trefines (MS asm_module (initial_asm_state main_asm))
-           (MS (imp_to_asm (dom _ main_asm) {["main"]} all_f2i imp_module)
-               (initial_imp_to_asm_state ∅ imp_module (initial_imp_state (<["main" := main_imp]> ∅)))).
-Proof.
-  apply: compile_correct; [|done|..].
-  - by vm_compute.
-  - by vm_compute.
-  - move => ??. rewrite /all_f2i !lookup_insert_Some !lookup_empty.
-    move => ?. destruct_all?; simplify_eq; compute_done.
-Qed.
-
-Global Instance seq_product_eq_dec : EqDecision seq_product_state.
-Proof. solve_decision. Qed.
-
 Inductive coro_prod_filter_state :=
 | CPFLeft (finit : option string) (started : bool)
 | CPFRight
 | CPFExited.
+
+Global Instance coro_prod_filter_state_inhabited : Inhabited coro_prod_filter_state := populate CPFRight.
 
 Definition coro_prod_filter (fns1 fns2 : gset string) : seq_product_state → coro_prod_filter_state → imp_ev → seq_product_state → coro_prod_filter_state → imp_ev → bool → Prop :=
   λ p s e p' s' e' ok,
@@ -360,7 +199,7 @@ Definition coro_prod_filter (fns1 fns2 : gset string) : seq_product_state → co
             ok = true
         end
     | CPFRight, _ =>
-        (* p must be SPRight: Not *)
+        (* p must be SPRight *)
         p = SPRight ∧
         match e with
         | EICall f vs h =>
@@ -398,66 +237,8 @@ Lemma coro_prod_trefines m1 m1' m2 m2' σ1 σ1' σ2 σ2' σ ins1 ins2 `{!VisNoAl
            (MS (coro_prod ins1 ins2 m1' m2') (σ, σ1', σ2')).
 Proof. move => ??. by apply mod_link_trefines. Qed.
 
-Definition yield_asm_dom : gset Z := locked (dom _) yield_asm.
+Ltac fast_set_solver := set_unfold; naive_solver.
 
-Definition initial_asm_prod_state (m1 m2 : module asm_event) (σ1 : m1.(m_state)) (σ2 : m2.(m_state)) :=
-  (@MLFNone asm_ev, @None seq_product_state, σ1, σ2).
-
-(* Definition coro_spec_inv m1 m2 *)
-(*   (σ1 : (asm_prod yield_asm_dom ∅ asm_module (imp_to_asm ∅ ∅ ∅ (imp_prod ∅ ∅  m1 m2))).(m_state)) *)
-(*   (σ2 : (imp_to_asm ∅ ∅ ∅ (coro_prod ∅ ∅ m1 m2)).(m_state)) : Prop := *)
-(*   let '(σa, σap, (AsmState i _ _ yins) , (σsm, (σi, cs, σi1, σi2), _)) := σ1 in *)
-(*   yins = yield_asm ∧ *)
-(*   i *)
-(*   . *)
-(*   → mod_link_state asm_ev * option seq_product_state * asm_state * *)
-(*     (mod_seq_map_state imp_event * (mod_link_state imp_ev * list seq_product_state * m_state m1 * m_state m2) * *)
-(*      (pp_state * imp_to_asm_state * uPred imp_to_asmUR)) *)
-(*     → mod_seq_map_state imp_event * (mod_link_state imp_ev * bool * m_state m1 * m_state m2) * *)
-(*       (pp_state * imp_to_asm_state * uPred imp_to_asmUR) → Prop *)
-
-
-  (* let 'Imp e1 h1 fns1' := σ1 in *)
-  (* let '(σf, cs, Imp el hl fnsl, Imp er hr fnsr) := σ2 in *)
-  (* ∃ n K Kl Kr e1' el' er' bl br, *)
-  (* fns1' = fns1 ∪ fns2 ∧ *)
-  (* fnsl = fns1 ∧ *)
-  (* fnsr = fns2 ∧ *)
-  (* imp_link_prod_combine_ectx n bl br σf cs K Kl Kr ∧ *)
-  (* e1 = expr_fill K e1' ∧ *)
-  (* el = expr_fill Kl el' ∧ *)
-  (* er = expr_fill Kr er' ∧ *)
-  (* match σf with *)
-  (* | MLFLeft => e1' = el' ∧ is_static_expr true el' ∧ er' = Waiting br ∧ h1 = hl *)
-  (*             ∧ (if bv then to_val el' = None else True) *)
-  (* | MLFRight => e1' = er' ∧ is_static_expr true er' ∧ el' = Waiting bl ∧ h1 = hr *)
-  (*              ∧ (if bv then to_val er' = None else True) *)
-  (* | MLFNone => e1' = Waiting (bl || br) ∧ el' = Waiting bl ∧ er' = Waiting br *)
-  (* | _ => False *)
-  (* end. *)
-
-Lemma i2a_mem_swap_stack sp1 gp1 sp2 gp2 mem:
-  i2a_mem_inv sp1 gp1 mem -∗
-  i2a_mem_stack sp2 gp2 -∗
-  i2a_mem_inv sp2 gp2 mem ∗ i2a_mem_stack sp1 gp1.
-Proof. iIntros "[??] ?". iFrame. Qed.
-
-Lemma i2a_mem_update_big sp gp mem mo mo' :
-  dom (gset _) mo = dom _ mo' →
-  i2a_mem_inv sp gp mem -∗
-  i2a_mem_map mo ==∗
-  i2a_mem_map mo' ∗ i2a_mem_inv sp gp (mo' ∪ mem).
-Proof.
-  iIntros (Hdom) "[$ Hmem] Hconst".
-  iMod (i2a_mem_delete_big' with "[$] [$]").
-  iMod (i2a_mem_alloc_big' with "[$]") as "[? $]".
-  { apply map_disjoint_spec => ???. rewrite !lookup_difference_Some -not_elem_of_dom Hdom not_elem_of_dom.  naive_solver. }
-  iModIntro.
-  by rewrite (map_difference_eq_dom_L _ mo mo') // -map_difference_union_r.
-Qed.
-
-(* We cannot use this lemma with imp_to_asm_combine since yield is not
-part of fns but parts of ins, but maybe we don't care? *)
 Theorem coro_spec m1 m2 σ1 σ2 ins1 ins2 fns1 fns2 f2i1 f2i2 finit regs_init gp_init
   `{!VisNoAll m1} `{!VisNoAll m2}:
   let fns := {["yield"]} ∪ fns1 ∪ fns2 in
@@ -475,8 +256,9 @@ Theorem coro_spec m1 m2 σ1 σ2 ins1 ins2 fns1 fns2 f2i1 f2i2 finit regs_init gp
   (∀ f, f ∈ fns1 → ∃ i, i ∈ ins1 ∧ f2i1 !! f = Some i) →
   (∀ f, f ∈ fns2 → ∃ i, i ∈ ins2 ∧ f2i2 !! f = Some i) →
   (∀ f i1 i2, f2i1 !! f = Some i1 → f2i2 !! f = Some i2 → i1 = i2) →
-  (∀ f i, f2i1 !! f = Some i → i ∈ ins2 → f ∈ fns2) →
-  (∀ f i, f2i2 !! f = Some i → i ∈ ins1 → f ∈ fns1) →
+  (∀ f i, f2i !! f = Some i → i ∈ ins2 → f ∈ fns2) →
+  (∀ f i, f2i !! f = Some i → i ∈ ins1 → f ∈ fns1) →
+  (∀ f i, f2i !! f = Some i → i ∈ yield_asm_dom → f = "yield") →
   i2a_mem_stack_mem (regs_init !!! "SP") gp_init ##ₘ coro_regs_mem regs_init →
   gp_init + GUARD_PAGE_SIZE ≤ regs_init !!! "SP" →
   trefines
@@ -492,8 +274,9 @@ Theorem coro_spec m1 m2 σ1 σ2 ins1 ins2 fns1 fns2 f2i1 f2i2 finit regs_init gp
           (initial_coro_prod_state finit _ _ σ1 σ2)))
 .
 Proof.
-  move => fns ins f2i mo Hinit Hfinit Hyf Hidisj Hfdisj Hydisj Hy1 Hy2 Hi1 Hi2 Hag Hf1 Hf2 Hmo Hgp.
-  have ? : ∀ f i1 i2, f2i1 !! f  = Some i1 → f2i !! f = Some i2 → i1 = i2. admit.
+  move => fns ins f2i mo Hinit Hfinit Hyf Hidisj Hfdisj Hydisj Hy1 Hy2 Hi1 Hi2 Hag Hf1 Hf2 Hfy Hmo Hgp.
+  have ? : ∀ f i1 i2, f2i1 !! f  = Some i1 → f2i !! f = Some i2 → i1 = i2.
+  { move => ???. rewrite /f2i lookup_union_Some_raw. naive_solver. }
   etrans. { apply: asm_prod_trefines; [|done]. apply (yield_asm_refines_itree regs_init). }
   apply: tsim_implies_trefines => n0 /=.
   tstep_i => *. case_match; destruct_all?; simplify_eq/=.
@@ -502,13 +285,13 @@ Proof.
   tstep_s. split!.
   tstep_s => ?.
   have ? : regs !!! "PC" ∈ ins1. { efeed pose proof Hi1; [done|]. destruct_all?. simplify_eq. naive_solver. }
-  rewrite bool_decide_false; [|set_solver].
-  rewrite bool_decide_true; [|set_solver].
+  rewrite bool_decide_false; [|fast_set_solver].
+  rewrite bool_decide_true; [|fast_set_solver].
   tstep_i => *. case_match; destruct_all?; simplify_eq/=.
-  rewrite bool_decide_true; [|set_solver].
+  rewrite bool_decide_true; [|fast_set_solver].
   tstep_i => *. simplify_eq.
   tstep_i. eexists true. split; [done|]. eexists h, gp, vs, avs, ret, f.
-  split!. {  admit. (* naive_solver. *) } { set_solver. }
+  split!. { naive_solver. } { fast_set_solver. }
   { iSatMono. iIntros!. rewrite /i2a_mem_map/mo big_sepM_empty big_sepM_union //. iDestruct!. iFrame.
     iDestruct (i2a_mem_stack_init with "[$]") as "?"; [done|]. iAccu. }
   tsim_mirror m1 σ1. move => ??? Hcont.
@@ -549,10 +332,11 @@ Proof.
                 cs2 = [I2AI true (yregs !!! "PC") regs1; I2AI false ret2 regs2] ∧
                 map_preserved saved_registers regs1 yregs) ∧
            σlc = MLFLeft ∧
+           yregs !!! "PC" ∈ ins2 ∧
            (if finit is Some f then f2i2 !! f = Some (yregs !!! "PC") ∧ f ∈ fns2 else True)
        (* Right side *)
        | CPFRight =>
-           ∃ gp ret2 regs1 regs2,
+           ∃ gp regs1 ret2 regs2,
            σpc1 = MLFRight ∧
            σsm1 = SMFilter ∧
            pp1 = PPOutside ∧
@@ -563,11 +347,13 @@ Proof.
            σsm2 = SMProg ∧
            pp2 = PPInside ∧
            cs2 = [I2AI false ret2 regs2] ∧
-           σlc = MLFRight
+           σlc = MLFRight ∧
+           yregs !!! "PC" ∈ ins1
        | _ => False
        end). }
-  { split!. { iSplit; iIntros!; iFrame. by iApply big_sepM_empty. } } { done. }
-  clear -Hyf Hidisj Hfdisj Hydisj Hy1 Hy2 Hi1 Hi2 Hag Hf1 Hf2 VisNoAll0 VisNoAll1.
+  { split!. { iSplit; iIntros!; iFrame. by iApply big_sepM_empty. } naive_solver. } { done. }
+  clear -Hyf Hidisj Hfdisj Hydisj Hy1 Hy2 Hi1 Hi2 Hag Hf1 Hf2 Hfy VisNoAll0 VisNoAll1.
+  have ? : yield_addr ∈ yield_asm_dom by rewrite /yield_asm_dom /yield_asm; unlock; compute_done.
   move => n ? Hloop [[[σpy1 σpy2][yt yregs]][[[σpc1 σpc2][[σsm1 σ1][[pp1 [cs1 lr1]]x1]]][[σsm2 σ2][[pp2 [cs2 lr2]]x2]]]].
   move => [[σsm' [[[σlc σc] σ1'] σ2']][[ppc [csc lrc]] xc]] [state ?]. destruct_all?; simplify_eq.
   destruct σc as [finit| |] => //; destruct_all?; simplify_eq.
@@ -583,10 +369,10 @@ Proof.
     + (* left to right *)
       tstep_s => ?.
       tstep_i => *. destruct_all?; simplify_map_eq'.
-      rewrite bool_decide_false. 2: set_solver.
-      rewrite bool_decide_false. 2: admit. (* 2: set_solver. *)
+      rewrite bool_decide_false. 2: fast_set_solver.
+      rewrite bool_decide_false. 2: fast_set_solver.
       move => /= *. destruct_all?; simplify_map_eq'.
-      rewrite bool_decide_true. 2: rewrite /yield_asm_dom; unlock; admit.
+      rewrite bool_decide_true; [|done].
       tstep_i. rewrite -/yield_itree. go.
       go_i => -[??]. go.
       go_i => ?. simplify_eq. go.
@@ -602,87 +388,23 @@ Proof.
       go_i => ?. go.
       go_i => *. destruct_all?. simplify_map_eq'. go.
       rewrite (coro_regs_regs_lookup_in "PC"); [|compute_done].
-      rewrite bool_decide_false. 2: admit.
-      rewrite bool_decide_true. 2: admit.
+      rewrite bool_decide_false. 2: fast_set_solver.
+      rewrite bool_decide_true. 2: fast_set_solver.
       tstep_i => *. destruct_all?; simplify_eq/=. destruct_all?; simplify_map_eq'.
       rewrite (coro_regs_regs_lookup_in "PC"); [|compute_done].
-      rewrite bool_decide_false. 2: admit.
-      rewrite bool_decide_true. 2: admit.
+      rewrite bool_decide_false. 2: fast_set_solver.
+      rewrite bool_decide_true. 2: fast_set_solver.
       tstep_i => *. simplify_eq.
       tstep_i.
       destruct finit; destruct_all?; simplify_eq.
       * eexists true. split!.
-        Set Nested Proofs Allowed.
-Lemma i2a_args_pure_mono o avs rs rs':
-  map_preserved args_registers rs rs' →
-  i2a_args_pure o avs rs →
-  i2a_args_pure o avs rs'.
-Proof.
-  move => Hrs Ha ???. have [?[??]]:= Ha _ _ ltac:(done). split!.
-  etrans; [|done].
-  symmetry. apply: Hrs. by apply: elem_of_list_lookup_2.
-Qed.
-Lemma coro_regs_regs_args_preserved rs rs':
- map_preserved args_registers rs (coro_regs_regs rs' ∪ rs).
-Proof.
-  rewrite /coro_regs_regs/=.
-  Transparent coro_saved_regs.
-  cbn.
-  rewrite -!insert_union_l left_id_L.
-  repeat (apply map_preserved_insert_r_not_in; [compute_done|]).
-  Opaque coro_saved_regs.
-  done.
-Qed.
-Lemma coro_regs_regs_touched_scramble rs rs' rs'':
-  map_scramble touched_registers rs rs' →
-  map_scramble touched_registers rs (coro_regs_regs rs'' ∪ rs').
-Proof.
-  move => ?.
-  rewrite /coro_regs_regs/=.
-  Transparent coro_saved_regs.
-  cbn.
-  rewrite -!insert_union_l left_id_L.
-  repeat (apply map_scramble_insert_r_in; [compute_done|]).
-  Opaque coro_saved_regs.
-  done.
-Qed.
-Lemma map_preserved_nil' {K A} `{Countable K} `{!Inhabited A} (m m' : gmap K A) ns:
-  ns = [] →
-  map_preserved ns m m'.
-Proof. move => -> ??. set_solver. Qed.
-
-Lemma coro_regs_regs_saved_preserved rs rs' rs'':
-  map_preserved saved_registers rs rs'' →
-  map_preserved saved_registers rs (coro_regs_regs rs'' ∪ rs').
-Proof.
-  move => Hp.
-  rewrite /coro_regs_regs/=.
-  Transparent coro_saved_regs.
-  cbn.
-  rewrite -!insert_union_l left_id_L.
-  apply map_preserved_insert_r_not_in; [compute_done|].
-  repeat (apply map_preserved_insert_r_in; [compute_done|]; split; [apply: Hp; compute_done|]).
-  apply map_preserved_nil'. compute_done.
-  Opaque coro_saved_regs.
-Qed.
-
-Lemma coro_regs_mem_dom rs rs':
-  dom (gset Z) (coro_regs_mem rs) = dom (gset Z) (coro_regs_mem rs').
-Proof.
-  rewrite /coro_regs_mem/coro_get_regs.
-  Transparent coro_saved_regs.
-  cbn. rewrite !dom_insert_L. done.
-  Opaque coro_saved_regs.
-Qed.
-
-
         { apply: i2a_args_pure_mono; [|done].
           apply map_preserved_insert_r_not_in; [compute_done|].
           apply map_preserved_insert_r_not_in; [compute_done|].
           apply coro_regs_regs_args_preserved. } { done. }
         { simplify_map_eq'. rewrite (coro_regs_regs_lookup_in "PC"); [|compute_done]. done. }
         2: { rewrite /i2a_regs_call. simplify_map_eq'. apply (coro_regs_regs_lookup_not_in "R30"). compute_done. }
-        { unfold i2a_regs_call in *. simplify_map_eq'. set_unfold. naive_solver. }
+        { unfold i2a_regs_call in *. simplify_map_eq'. fast_set_solver. }
         { iSatMonoBupd. iFrame. simplify_map_eq'.
           rewrite (coro_regs_regs_lookup_in "SP"); [|compute_done].
           iDestruct (i2a_mem_swap_stack with "Hm [$]") as "[Hm ?]".
@@ -702,6 +424,7 @@ Qed.
           apply map_scramble_insert_r_in; [compute_done|].
           by apply coro_regs_regs_touched_scramble. }
         { simplify_map_eq'. iSplit; iIntros!; iFrame. }
+        { unfold i2a_regs_call in *. simplify_map_eq'. done. }
       * destruct args as [|? [|]] => //.
         eexists false. split!.
         { simplify_map_eq'. rewrite (coro_regs_regs_lookup_in "PC"); [|compute_done]. done. }
@@ -730,17 +453,24 @@ Qed.
           apply map_scramble_insert_r_in; [compute_done|].
           by apply coro_regs_regs_touched_scramble. }
         { simplify_map_eq'. iSplit; iIntros!; iFrame. }
+        { unfold i2a_regs_call in *. simplify_map_eq'. done. }
     + (* left call to outside *)
       case_bool_decide; [by tstep_s|].
       rewrite bool_decide_true //=.
-      tstep_i => *. destruct_all?; simplify_eq.
-      rewrite bool_decide_false. 2: admit.
-      rewrite bool_decide_false. 2: admit.
+      tstep_i => ? rs *. destruct_all?; simplify_eq.
+      have ?: rs !!! "PC" ∉ ins. {
+        set_unfold => -[[?|?]|?].
+        - efeed pose proof Hfy; [apply lookup_union_Some_raw; naive_solver|done|done].
+        - efeed pose proof Hf2; [apply lookup_union_Some_raw; naive_solver|done|done].
+        - efeed pose proof Hf1; [apply lookup_union_Some_raw; naive_solver|done|done].
+      }
+      rewrite bool_decide_false. 2: fast_set_solver.
+      rewrite bool_decide_false. 2: fast_set_solver.
       move => /= *. destruct_all?; simplify_eq/=.
-      rewrite bool_decide_false. 2: admit.
-      rewrite bool_decide_false. 2: admit.
-      tstep_s. split!. done. set_solver. admit. 2: done. set_solver.
-      { by etrans. }
+      rewrite bool_decide_false. 2: fast_set_solver.
+      rewrite bool_decide_false. 2: fast_set_solver.
+      tstep_s. split!. { done. } { fast_set_solver. } { apply lookup_union_Some_raw. naive_solver. }
+      { fast_set_solver. }
       { iSatMono. setoid_subst. iIntros!. iFrame. iAccu. }
       iSatClear.
 
@@ -749,12 +479,12 @@ Qed.
       tstep_s. split!.
       tstep_s => -[] /= *. { tstep_s. split!. by tstep_s. }
       tstep_s. split!. destruct_all?; simplify_eq.
-      rewrite bool_decide_false. 2: admit.
-      rewrite bool_decide_true. 2: set_solver.
+      rewrite bool_decide_false. 2: fast_set_solver.
+      rewrite bool_decide_true. 2: fast_set_solver.
       tstep_i => /= *. destruct_all?; simplify_eq/=. destruct_all?; simplify_eq/=.
       rewrite bool_decide_true; [|done].
       tstep_i => *. simplify_eq.
-      tstep_i => *. eexists false. split!. done.
+      tstep_i => *. eexists false. split!.
       { iSatMono. iIntros!. iFrame. iAccu. }
       tsim_mirror m1 σ' => ??? Hcont.
       tstep_both. apply Hcont => -[?|] ?? Hs *. simplify_eq.
@@ -765,13 +495,12 @@ Qed.
       split!. iSplit; iIntros!; iFrame.
     + (* left return to outside *)
       tstep_i => *. destruct_all?; simplify_eq.
-      rewrite bool_decide_false. 2: set_solver.
-      rewrite bool_decide_false. 2: set_solver.
+      rewrite bool_decide_false. 2: fast_set_solver.
+      rewrite bool_decide_false. 2: fast_set_solver.
       move => /= *. destruct_all?; simplify_eq/=.
-      rewrite bool_decide_false. 2: set_solver.
-      rewrite bool_decide_false. 2: set_solver.
-      tstep_s. split!. done.
-      { by etrans. }
+      rewrite bool_decide_false. 2: fast_set_solver.
+      rewrite bool_decide_false. 2: fast_set_solver.
+      tstep_s. split!.
       { iSatMono. setoid_subst. iIntros!. iFrame. iAccu. }
       iSatClear.
 
@@ -790,10 +519,10 @@ Qed.
     + (* right to left *)
       tstep_s => ?.
       tstep_i => *. destruct_all?; simplify_map_eq'.
-      rewrite bool_decide_false. 2: admit.
-      rewrite bool_decide_false. 2: admit. (* 2: set_solver. *)
+      rewrite bool_decide_false. 2: fast_set_solver.
+      rewrite bool_decide_false. 2: fast_set_solver.
       move => /= *. destruct_all?; simplify_map_eq'.
-      rewrite bool_decide_true. 2: rewrite /yield_asm_dom; unlock; admit.
+      rewrite bool_decide_true. 2: done.
       tstep_i. rewrite -/yield_itree. go.
       go_i => -[??]. go.
       go_i => ?. simplify_eq. go.
@@ -809,11 +538,11 @@ Qed.
       go_i => ?. go.
       go_i => *. destruct_all?. simplify_map_eq'. go.
       rewrite (coro_regs_regs_lookup_in "PC"); [|compute_done].
-      rewrite bool_decide_false. 2: admit.
-      rewrite bool_decide_true. 2: admit.
+      rewrite bool_decide_false. 2: fast_set_solver.
+      rewrite bool_decide_true. 2: fast_set_solver.
       tstep_i => *. destruct_all?; simplify_eq/=. destruct_all?; simplify_map_eq'.
       rewrite (coro_regs_regs_lookup_in "PC"); [|compute_done].
-      rewrite bool_decide_true. 2: admit.
+      rewrite bool_decide_true. 2: fast_set_solver.
       tstep_i => *. simplify_eq.
       tstep_i.
       destruct args as [|? [|]] => //.
@@ -844,17 +573,27 @@ Qed.
       { simplify_map_eq'. iSplit; iIntros!; iFrame. }
       { simplify_map_eq'. revert select (i2a_regs_call _ _) => ->. done. }
       { apply map_preserved_insert_r_not_in; [compute_done|]. done. }
+      { unfold i2a_regs_call in *. simplify_map_eq'. done. }
     + (* right call to outside *)
       case_bool_decide; [by tstep_s|].
       rewrite bool_decide_true //=.
-      tstep_i => *. destruct_all?; simplify_eq.
-      rewrite bool_decide_false. 2: admit.
-      rewrite bool_decide_false. 2: admit.
+      tstep_i => ? rs *. destruct_all?; simplify_eq.
+      have ? : f2i !! fn = Some (rs !!! "PC"). {
+        apply lookup_union_Some_raw.
+        destruct (f2i1 !! fn) eqn:?; naive_solver.
+      }
+      have ?: rs !!! "PC" ∉ ins. {
+        set_unfold => -[[?|?]|?].
+        - efeed pose proof Hfy; [done|done|done].
+        - efeed pose proof Hf2; [done|done|done].
+        - efeed pose proof Hf1; [done|done|done].
+      }
+      rewrite bool_decide_false. 2: fast_set_solver.
+      rewrite bool_decide_false. 2: fast_set_solver.
       move => /= *. destruct_all?; simplify_eq/=.
-      rewrite bool_decide_false. 2: admit.
-      rewrite bool_decide_false. 2: admit.
-      tstep_s. split!. done. set_solver. admit. 2: done. set_solver.
-      { by etrans. }
+      rewrite bool_decide_false. 2: fast_set_solver.
+      rewrite bool_decide_false. 2: fast_set_solver.
+      tstep_s. split!. { done. } { fast_set_solver. } { fast_set_solver. }
       { iSatMono. setoid_subst. iIntros!. iFrame. iAccu. }
       iSatClear.
 
@@ -863,13 +602,13 @@ Qed.
       tstep_s. split!.
       tstep_s => -[] /= *. { tstep_s. split!. by tstep_s. }
       tstep_s. split!. destruct_all?; simplify_eq.
-      rewrite bool_decide_false. 2: admit.
-      rewrite bool_decide_true. 2: set_solver.
+      rewrite bool_decide_false. 2: fast_set_solver.
+      rewrite bool_decide_true. 2: fast_set_solver.
       tstep_i => /= *. destruct_all?; simplify_eq/=. destruct_all?; simplify_eq/=.
-      rewrite bool_decide_false. 2: set_solver.
+      rewrite bool_decide_false. 2: fast_set_solver.
       rewrite bool_decide_true; [|done].
       tstep_i => *. simplify_eq.
-      tstep_i => *. eexists false. split!. done.
+      tstep_i => *. eexists false. split!.
       { iSatMono. iIntros!. iFrame. iAccu. }
       tsim_mirror m2 σ' => ??? Hcont.
       tstep_both. apply Hcont => -[?|] ?? Hs *. simplify_eq.
@@ -879,4 +618,6 @@ Qed.
       apply: Hloop. { etrans; [|done]. etrans; [|done]. apply ti_le_S. }
       split!. iSplit; iIntros!; iFrame.
     + (* right return to outside *) by tstep_s.
-Abort.
+ Unshelve.
+ all: apply: inhabitant.
+Qed.
