theories/coroutine_example.v
@@ -1,0 +1,95 @@
+Require Export refframe.module.
+Require Import refframe.trefines.
+Require Import refframe.filter.
+Require Import refframe.product.
+Require Import refframe.seq_product.
+Require Import refframe.link.
+Require Import refframe.proof_techniques.
+Require Import refframe.prepost.
+Require Import refframe.imp.
+Require Import refframe.asm.
+Require Import refframe.itree.
+Require Import refframe.imp_to_asm.
+Require Import refframe.coroutine.
+Require Import refframe.compiler.compiler.
+
+(***
+void stream_inner(int n) {
+  gtyield_with_val(n);
+  stream_inner(n+1);
+}
+
+void stream()
+{
+  stream_inner(0);
+}
+
+int main(void)
+{
+  gtgo(stream);
+  for(int i=0; i<5; i++) {
+    int v = gtyield_with_val(-1);
+    printf("v is : %d\n", v);
+  }
+}
+***)
+
+Definition stream_addr: Z := 400.
+Definition main_addr: Z := 500.
+Definition print_addr: Z := 600.
+
+Definition stream_imp: fndef := {|
+  fd_args := [("n")];
+  fd_vars := [];
+  fd_body := LetE "_" (imp.Call "yield" [Var "n"]) $
+             (imp.Call "stream" [(BinOp (Var "n") AddOp (Val $ ValNum 1))]);
+  fd_static := I
+|}.
+
+Definition main_imp: fndef := {|
+  fd_args := [];
+  fd_vars := [];
+  fd_body := LetE "x" (imp.Call "yield" [Val $ ValNum 0]) $
+             LetE "_" (imp.Call "print" [(Var "x")]) $
+             LetE "y" (imp.Call "yield" [Val $ ValNum 0]) $
+             LetE "_" (imp.Call "print" [(Var "y")]) $
+             (Val $ ValNum (-1));
+  fd_static := I
+|}.
+
+Definition all_f2i : gmap string Z :=
+  <["yield"  := yield_addr]> $
+  <["stream" := stream_addr]> $
+  <["main"   := main_addr]> $
+  <["print"  := print_addr]> $
+  ∅.
+
+Definition stream_asm : gmap Z asm_instr :=
+  deep_to_asm_instrs stream_addr ltac:(i2a_compile all_f2i stream_imp).
+
+Definition main_asm : gmap Z asm_instr :=
+  deep_to_asm_instrs main_addr ltac:(i2a_compile all_f2i main_imp).
+
+Lemma stream_asm_refines_imp :
+  trefines (MS asm_module (initial_asm_state stream_asm))
+           (MS (imp_to_asm (dom _ stream_asm) {["stream"]} all_f2i imp_module)
+               (initial_imp_to_asm_state ∅ imp_module (initial_imp_state (<["stream" := stream_imp]> ∅)))).
+Proof.
+  apply: compile_correct; [|done|..].
+  - by vm_compute.
+  - by vm_compute.
+  - move => ??. rewrite /all_f2i !lookup_insert_Some !lookup_empty.
+    move => ?. destruct_all?; simplify_eq; compute_done.
+Qed.
+
+Lemma main_asm_refines_imp :
+  trefines (MS asm_module (initial_asm_state main_asm))
+           (MS (imp_to_asm (dom _ main_asm) {["main"]} all_f2i imp_module)
+               (initial_imp_to_asm_state ∅ imp_module (initial_imp_state (<["main" := main_imp]> ∅)))).
+Proof.
+  apply: compile_correct; [|done|..].
+  - by vm_compute.
+  - by vm_compute.
+  - move => ??. rewrite /all_f2i !lookup_insert_Some !lookup_empty.
+    move => ?. destruct_all?; simplify_eq; compute_done.
+Qed.
