theories/print.v
@@ -1,0 +1,88 @@
+Require Export refframe.module.
+Require Import refframe.trefines.
+Require Import refframe.filter.
+Require Import refframe.product.
+Require Import refframe.seq_product.
+Require Import refframe.link.
+Require Import refframe.proof_techniques.
+Require Import refframe.prepost.
+Require Import refframe.imp.
+Require Import refframe.asm.
+Require Import refframe.itree.
+Require Import refframe.imp_to_asm.
+
+Local Open Scope Z_scope.
+
+Definition __NR_PRINT : Z := 42.
+Definition print_addr : Z := 500.
+
+Definition print_asm : gmap Z asm_instr :=
+  deep_to_asm_instrs print_addr [
+      Amov "R8" (ImmediateOp __NR_PRINT);
+      ASyscall;
+      Aret
+    ].
+
+Definition print_itree : itree (moduleE asm_event unit) unit :=
+  ITree.forever (
+    '(rs, mem) ← TReceive (λ '(rs, mem), (Incoming, EAJump rs mem));;;
+    TAssume (rs !!! "PC" = print_addr);;;;
+    TAssume (print_asm !! (rs !!! "R30") = None);;;;
+    args ← TExist _;;;
+    TAssert (length args = length syscall_arg_regs);;;;
+    TAssert (args !! 0%nat = Some (rs !!! "R0"));;;;
+    TAssert (args !! 8%nat = Some __NR_PRINT);;;;
+    TVis (Outgoing, EASyscallCall args);;;;
+    ret ← TReceive (λ ret, (Incoming, EASyscallRet ret));;;
+    TVis (Outgoing, EAJump (<["PC" := rs !!! "R30"]> $
+                            <["R0" := ret]> $
+                            <["R8" := __NR_PRINT]> $
+                            rs) mem)).
+
+Local Ltac go :=
+  clear_itree.
+Local Ltac go_s :=
+  tstep_s; go.
+Local Ltac go_i :=
+  tstep_i; go.
+
+Lemma print_asm_refines_itree :
+  trefines (MS asm_module (initial_asm_state print_asm))
+           (MS (mod_itree _ _) (print_itree, tt)).
+Proof.
+  apply: tsim_implies_trefines => n0 /=.
+  unshelve eapply tsim_remember. { simpl. exact (λ _ σa '(t, _),
+    t ≈ print_itree ∧
+    σa.(asm_cur_instr) = AWaiting ∧
+    σa.(asm_instrs) = print_asm). }
+  { split!. } { done. }
+  move => n _ Hloop [????] [??] ?. destruct_all?; simplify_eq/=.
+  tstep_i => ????? Hi. tstep_s. rewrite -/print_itree. go.
+  go_s. eexists (_, _). go.
+  go_s. split!. go.
+  go_s => ?. go.
+  go_s => ?. go.
+  tstep_i => ??. simplify_map_eq'.
+  tstep_i.
+  tstep_i.
+  tstep_i => ??. simplify_map_eq'.
+  tstep_i.
+  go_s. eexists _. go.
+  go_s. split; [shelve|]. go.
+  go_s. split; [shelve|]. go.
+  go_s. split; [shelve|]. go.
+  go_s. split!. go.
+  tstep_i => ?.
+  go_s. eexists _. go.
+  go_s. split!. go.
+  tstep_i.
+  tstep_i => ??. simplify_map_eq'.
+  tstep_i. simplify_map_eq'.
+  tstep_i => ??. simplify_map_eq'.
+  go_s. sort_map_insert. simplify_map_eq'. split!. go.
+  by apply: Hloop.
+  Unshelve.
+  - done.
+  - by simplify_map_eq'.
+  - by simplify_map_eq'.
+Qed.
